@prefix cov: <https://www.w3.org/2019/wot/coap#> .
@prefix dcterms: <http://purl.org/dc/terms/> .
@prefix owl: <http://www.w3.org/2002/07/owl#> .
@prefix rdf: <http://www.w3.org/1999/02/22-rdf-syntax-ns#> .
@prefix rdfs: <http://www.w3.org/2000/01/rdf-schema#> .
@prefix schema: <http://schema.org/> .
@prefix vann: <http://purl.org/vocab/vann/> .
@prefix xsd: <http://www.w3.org/2001/XMLSchema#> .
@base <https://www.w3.org/2019/wot/coap> .

<> a owl:Ontology ;
   dcterms:title "CoAP Vocabulary for the Web of Things"@en ;
   rdfs:label "CoAP Vocabulary for the Web of Things"@en ; # TODO: Refactor
   dcterms:creator [ a dcterms:Agent ,
                       schema:Person ;
                     schema:name "Klaus Hartke" ;
                     schema:affiliation [ a schema:Organization ;
                                          schema:name "Siemens AG" ;
                                          schema:url "https://www.siemens.com/"
                                        ]
                   ] ,
                   [ a dcterms:Agent ,
                       schema:Person ;
                     schema:name "Jan Romann" ;
                     schema:affiliation [ a schema:Organization ;
                                          schema:name "Invited Expert" ;
                                          schema:url "https://github.com/JKRhb/"
                                        ]
                   ] ;
   vann:preferredNamespacePrefix "cov" ;
   vann:preferredNamespaceUri "https://www.w3.org/2019/wot/coap#" ;
   rdfs:comment "This document contains RDF Vocabulary that can be used in CoAP forms of Web of Things Thing Descriptions." .

cov:method a rdf:Property, owl:DatatypeProperty ;
           rdfs:range xsd:string ;
           rdfs:comment "Indicates the CoAP method to be used in the request."@en ;
           rdfs:isDefinedBy <> ;
           rdfs:seeAlso "See the <a href=\"https://www.iana.org/assignments/core-parameters/#method-codes\">CoAP Method Codes</a> registry for the set of possible values.";
           rdfs:label "method"@en .

cov:blockwise a rdf:Property, owl:ObjectProperty ;
              rdfs:range cov:BlockWiseTransferParameters ;
              rdfs:comment "Indicates that block-wise transfer [[RFC7959]] is supported."@en ;
              rdfs:isDefinedBy <> ;
              rdfs:label "blockwise"@en .

cov:qblockwise a rdf:Property, owl:ObjectProperty ;
               rdfs:range cov:BlockWiseTransferParameters ;
               rdfs:comment "Indicates that quick block-wise transfer [[RFC9177]] is supported."@en ;
               rdfs:isDefinedBy <> ;
               rdfs:label "qblockwise"@en .

cov:hopLimit a rdf:Property, owl:DatatypeProperty ;
             rdfs:range xsd:unsignedByte ;
             rdfs:comment "Indicates that a CoAP Hop-Limit option [[RFC8768]] should be included in the request."@en ;
             rdfs:isDefinedBy <> ;
             rdfs:label "hopLimit"@en .

cov:contentFormat a rdf:Property, owl:DatatypeProperty ;
                  rdfs:range xsd:unsignedShort ;
                  rdfs:comment "Indicates a numeric CoAP Content-Format [[RFC7252]] as a combination of Media Type and Content Coding. Must match the given <code>contentType</code> and <code>contentCoding</code> members."@en ;
                  rdfs:isDefinedBy <> ;
                  rdfs:label "contentFormat"@en .

cov:accept a rdf:Property, owl:DatatypeProperty ;
           rdfs:range xsd:unsignedShort ;
           rdfs:comment "Indicates that a Consumer must include an Accept option [[RFC7252]] with the given value when requesting the resource associated with this Form."@en ;
           rdfs:isDefinedBy <> ;
           rdfs:label "accept"@en .

cov:block2Size a rdf:Property, owl:DatatypeProperty ;
               rdfs:domain cov:BlockWiseTransferParameters ;
               schema:domainIncludes cov:BlockWiseTransferParameters ;
               rdfs:range xsd:unsignedShort ;
               rdfs:comment "Indicates the largest block size that may be used in a Block2 or Q-Block2 Option"@en ;
               rdfs:label "block2Size"@en .

cov:block1Size a rdf:Property, owl:DatatypeProperty ;
               rdfs:domain cov:BlockWiseTransferParameters ;
               schema:domainIncludes cov:BlockWiseTransferParameters ;
               rdfs:range xsd:unsignedShort ;
               rdfs:comment "Indicates the largest block size that may be used in a Block1 or Q-Block1 Option"@en ;
               rdfs:label "block1Size"@en .

cov:BlockWiseTransferParameters a rdfs:Class, owl:Class ;
                                rdfs:isDefinedBy <> ;
                                rdfs:comment "Parameters used for block-wise transfer [[RFC7959]] and block-wise transfer supporting robust transmission [[RFC9177]]."@en ;
                                rdfs:label "BlockWiseTransferParameters"@en .
