@prefix : <https://www.w3.org/2019/wot/mqtt#> .
@prefix dct: <http://purl.org/dc/terms/> .
@prefix owl: <http://www.w3.org/2002/07/owl#> .
@prefix rdf: <http://www.w3.org/1999/02/22-rdf-syntax-ns#> .
@prefix xml: <http://www.w3.org/XML/1998/namespace> .
@prefix xsd: <http://www.w3.org/2001/XMLSchema#> .
@prefix rdfs: <http://www.w3.org/2000/01/rdf-schema#> .
@prefix vann: <http://purl.org/vocab/vann/> .
@prefix schema: <http://schema.org/> .
@base <https://www.w3.org/2019/wot/mqtt> .


<https://www.w3.org/2019/wot/mqtt> rdf:type owl:Ontology ;
                                    dct:creator [ rdf:type schema:Person ;
                                                  schema:affiliation [ rdf:type schema:Organization ;
                                                                       schema:name "Invited Expert" ;
                                                                       schema:url "https://github.com/mjkoster/"
                                                                     ] ;
                                                  schema:name "Michael Koster"
                                                ] ;
                                    dct:contributor <https://www.vcharpenay.link/#me> ,
                                                    [ rdf:type schema:Person ;
                                                      schema:affiliation _:genid4 ;
                                                      schema:name "Ege Korkan"
                                                    ] ,
                                                    [ rdf:type schema:Person ;
                                                      schema:affiliation _:genid4 ;
                                                      schema:name "Sebastian Käbisch"
                                                    ] ;
                                    vann:preferredNamespacePrefix "mqv" ;
                                    vann:preferredNamespaceUri : ;
                                    rdfs:comment "Vocabulary to represent MQTT packets in RDF."@en ;
                                    rdfs:label "MQTT in RDF"@en .

_:genid4 rdf:type schema:Organization ;
          schema:name "Siemens AG" ;
          schema:url "https://www.siemens.com/" .

#################################################################
#    Object Properties
#################################################################

###  https://www.w3.org/2019/wot/mqtt#sendsControlPacket
:sendsControlPacket rdf:type owl:ObjectProperty ;
    rdfs:label "sendsControlPacket"@en ;
    rdfs:comment """In MQTT protocol clients sends <a href='https://w3c.github.io/wot-binding-templates/ontology/mqtt#control-packet'>control packet</a>s between each other using and intermediary called Server (or broker). 
    This property describes the action of sending a <a href='https://w3c.github.io/wot-binding-templates/ontology/mqtt#control-packet'>ControlPacket</a> in a <a href='https://w3c.github.io/wot-binding-templates/ontology/mqtt#network-connection'>NetworkConnection</a>"""@en ;
    rdfs:range :ControlPacket ;
    rdfs:domain :Client .

###  https://www.w3.org/2019/wot/mqtt#hasQoSFlag
:hasQoSFlag rdf:type owl:ObjectProperty ;
               rdfs:domain :SUBSCRIBE ;
               rdfs:range :QualityOfService ;
               schema:domainIncludes :SUBSCRIBE ;
               rdfs:comment "This field indicates the level of assurance for delivery of an Application Message."@en ;
               rdfs:isDefinedBy <https://www.w3.org/2019/wot/mqtt> ;
               rdfs:label "hasQoSFlag"@en .

###  https://www.w3.org/2019/wot/mqtt#hasPayload
:hasPayload rdf:type owl:ObjectProperty ;
            rdfs:range :ControlPacket ;
            schema:domainIncludes :ControlPacket ;
            rdfs:comment "Some MQTT Control Packets contain a Payload as the final part of the packet. In the PUBLISH packet this is the Application Message."@en ;
            rdfs:isDefinedBy <https://www.w3.org/2019/wot/mqtt> ;
            rdfs:label "hasPayload"@en .

###  https://www.w3.org/2019/wot/mqtt#hasTopicName
:hasTopicName rdf:type owl:ObjectProperty ;
                rdfs:domain :PUBLISH ;
                schema:domainIncludes :PUBLISH ;
                rdfs:comment "This field reports the <a href='https://w3c.github.io/wot-binding-templates/ontology/mqtt#topic-name'>TopicName</a> of a packet"@en ;
                rdfs:label "hasTopicName"@en ;
                schema:rangeIncludes :TopicName ;
                rdfs:range :TopicName .

###  https://www.w3.org/2019/wot/mqtt#hasTopicFilters
:hasTopicFilters rdf:type owl:ObjectProperty ;
                rdfs:domain :SUBSCRIBE, :UNSUBSCRIBE ;
                schema:domainIncludes :SUBSCRIBE, :UNSUBSCRIBE ;
                rdfs:comment "This field reports the list of <a href='https://w3c.github.io/wot-binding-templates/ontology/mqtt#topic-filter'>TopicFilter</a>s of a packet"@en ;
                rdfs:label "hasTopicFilters"@en ;
                schema:rangeIncludes :TopicFilter ;
                rdfs:range :TopicFilter .

#################################################################
#    Data properties
#################################################################

###  https://www.w3.org/2019/wot/mqtt#fixedHeaderFlag
:fixedHeaderFlag rdf:type owl:DatatypeProperty ;
                 schema:domainIncludes :ControlPacket ;
                 rdfs:comment "Each MQTT Control Packet contains a Fixed Header."@en ;
                 rdfs:isDefinedBy <https://www.w3.org/2019/wot/mqtt> ;
                 rdfs:label "fixedHeaderFlag"@en .


###  https://www.w3.org/2019/wot/mqtt#hasDUPFlaghasRetainFlag
:hasDUPFlag rdf:type owl:DatatypeProperty ;
            rdfs:subPropertyOf :fixedHeaderFlag ;
            schema:domainIncludes :SUBSCRIBE ;
            rdfs:range xsd:boolean ;
            rdfs:comment "If the DUP flag is set, it indicates that this might be re-delivery of an earlier attempt to send the packet."@en ;
            rdfs:isDefinedBy <https://www.w3.org/2019/wot/mqtt> ;
            rdfs:label "hasDUPFlag"@en .


###  https://www.w3.org/2019/wot/mqtt#hasRetainFlag
:hasRetainFlag rdf:type owl:DatatypeProperty ;
               rdfs:subPropertyOf :fixedHeaderFlag ;
               schema:domainIncludes :SUBSCRIBE ;
               rdfs:range xsd:boolean ;
               rdfs:comment "If the RETAIN flag is set to 1 in a PUBLISH packet sent by a Client to a Server, the Server must replace any existing retained message for this topic and store the Application Message, so that it can be delivered to future subscribers whose subscriptions match its Topic Name."@en ;
               rdfs:isDefinedBy <https://www.w3.org/2019/wot/mqtt> ;
               rdfs:label "hasRetainFlag"@en .


###  https://www.w3.org/2019/wot/mqtt#hasVariableHeaderFlag
:hasVariableHeaderFlag rdf:type owl:DatatypeProperty ;
                    schema:domainIncludes :ControlPacket ;
                    rdfs:comment "Some types of MQTT Control Packet contain a Variable Header component. It resides between the Fixed Header and the Payload. The content of the Variable Header varies depending on the packet type."@en ;
                    rdfs:isDefinedBy <https://www.w3.org/2019/wot/mqtt> ;
                    rdfs:label "hasVariableHeaderFlag"@en .


#################################################################
#    Classes
#################################################################

###  https://www.w3.org/2019/wot/mqtt#ControlPacket
:ControlPacket rdf:type owl:Class ;
               owl:equivalentClass [ rdf:type owl:Class ;
                                     owl:oneOf(
                                           :PUBLISH
                                           :SUBSCRIBE
                                           :UNSUBSCRIBE
                                     ) ] ;
               rdfs:comment "An MQTT Control Packet consists of up to three parts: fixed header (prsesent in all Control Packets), variable header, payload"@en ;
               rdfs:isDefinedBy <https://www.w3.org/2019/wot/mqtt> ;
               rdfs:label "Control Packet"@en .


###  https://www.w3.org/2019/wot/mqtt#PUBLISH
:PUBLISH rdf:type owl:Class ;
               rdfs:subClassOf :ControlPacket ;
               rdfs:comment "A PUBLISH packet is sent from a Client to a Server or from a Server to a Client to transport an Application Message."@en ;
               rdfs:isDefinedBy <https://www.w3.org/2019/wot/mqtt> ;
               rdfs:label "PublishPacket"@en .


###  https://www.w3.org/2019/wot/mqtt#SUBSCRIBE
:SUBSCRIBE rdf:type owl:Class ;
                 rdfs:subClassOf :ControlPacket ;
                 rdfs:comment "The SUBSCRIBE packet is sent from the Client to the Server to create one or more Subscriptions. Each Subscription registers a Client’s interest in one or more Topics."@en ;
                 rdfs:isDefinedBy <https://www.w3.org/2019/wot/mqtt> ;
                 rdfs:label "SubscribePacket"@en .


###  https://www.w3.org/2019/wot/mqtt#UNSUBSCRIBE
:UNSUBSCRIBE rdf:type owl:Class ;
                   rdfs:subClassOf :ControlPacket ;
                   rdfs:comment "An UNSUBSCRIBE packet is sent by the Client to the Server, to unsubscribe from topics."@en ;
                   rdfs:isDefinedBy <https://www.w3.org/2019/wot/mqtt> ;
                   rdfs:label "UnsubscribePacket"@en .


###  https://www.w3.org/2019/wot/mqtt#QualityOfService
:QualityOfService rdf:type owl:Class ;
                   owl:equivalentClass [ a owl:Class ;
                                         owl:oneOf ( <https://www.w3.org/2019/wot/mqtt/qualitfyOfService#0>
                                                     <https://www.w3.org/2019/wot/mqtt/qualitfyOfService#1>
                                                     <https://www.w3.org/2019/wot/mqtt/qualitfyOfService#2> ) ] ; 
                   rdfs:comment "MQTT delivers Application Messages according to the Quality of Service (QoS) levels defined in this ontology."@en ;
                   rdfs:isDefinedBy <https://www.w3.org/2019/wot/mqtt> ;
                   rdfs:label "QualityOfService"@en ;
                   schema:alternateName "QoS"@en .

###  https://www.w3.org/2019/wot/mqtt#TopicName
:TopicName rdf:type owl:Class ;
       rdfs:comment "The label attached to an Application Message which is matched against the Subscriptions known to the Server. The Server sends a copy of the Application Message to each Client that has a matching Subscription. TopicName is used only for publication to indicate a single topic, and thus MUST not contain any wildcards."@en ;
       rdfs:label "Topic Name"@en .

###  https://www.w3.org/2019/wot/mqtt#TopicFilter
:TopicFilter rdf:type owl:Class ;
       rdfs:comment "An expression contained in a Subscription, to indicate an interest in one or more topics. A Topic Filter can include wildcard characters. TopicFilter is used for subscriptions to indicate a topic or a set of topics when a wildcard character is used."@en ;
       rdfs:label "Topic Filter"@en .

###  https://www.w3.org/2019/wot/mqtt#NetworkConnection
:NetworkConnection rdf:type owl:Class ;
       rdfs:comment "The MQTT protocol requires an underlying transport that provides an ordered, lossless, stream of bytes from the Client to Server and Server to Client. See <a href='https://docs.oasis-open.org/mqtt/mqtt/v3.1.1/os/mqtt-v3.1.1-os.html#_Toc398718098'>NetworkConnection</a>"@en ;
       rdfs:label "Network Connection"@en .

###  https://www.w3.org/2019/wot/mqtt#Client
:Client rdf:type owl:Class ;
       rdfs:comment "A program or device that uses MQTT. A Client always establishes the <a href='#network-connection'>Network Connection</a> to a <a href='#server'>Server</a>"@en ;
       rdfs:label "Client"@en .

###  https://www.w3.org/2019/wot/mqtt#Server
:Server rdf:type owl:Class ;
       rdfs:comment "A program or device that acts as an intermediary between <a href='#client'>client</a>s. Sometimes servers are referred as Brokers"@en ;
       rdfs:label "Server"@en .
#################################################################
#    Individuals
#################################################################

###  https://www.vcharpenay.link/#me
<https://www.vcharpenay.link/#me> rdf:type owl:NamedIndividual ,
                                           schema:Person ;
                                  schema:affiliation _:genid4 ;
                                  schema:name "Victor Charpenay" .


###  https://www.w3.org/2019/wot/mqtt/qualitfyOfService#0
<https://www.w3.org/2019/wot/mqtt/qualitfyOfService#0> rdf:type owl:NamedIndividual ,
            :QualityOfService ;
            rdfs:comment "The Server delivers the Application Message to the Client at most once"@en ;
            rdfs:label "atMostOnce"@en ;
            rdfs:subClassOf :QualityOfService ;
            schema:alternateName "QoS0"@en ;
            rdfs:isDefinedBy <https://www.w3.org/2019/wot/mqtt> .

###  https://www.w3.org/2019/wot/mqtt/qualitfyOfService#atLeastOnce
<https://www.w3.org/2019/wot/mqtt/qualitfyOfService#1> rdf:type owl:NamedIndividual ,
              :QualityOfService ;
              rdfs:comment "The message is delivered at least once."@en ;
              rdfs:label "atLeastOnce"@en ;
              schema:alternateName "QoS1"@en ;
              rdfs:subClassOf :QualityOfService ;
              rdfs:isDefinedBy <https://www.w3.org/2019/wot/mqtt> .

###  https://www.w3.org/2019/wot/mqtt/qualitfyOfService#exactlyOnce
<https://www.w3.org/2019/wot/mqtt/qualitfyOfService#2> rdf:type owl:NamedIndividual ,
             :QualityOfService ;
             rdfs:comment "The message is delivered exactly once."@en ;
             rdfs:label "exactlyOnce"@en ;
             schema:alternateName "QoS2"@en ;
             rdfs:subClassOf :QualityOfService ;
             rdfs:isDefinedBy <https://www.w3.org/2019/wot/mqtt> .
###  Generated by the OWL API (version 4.5.7.2018-12-02T02:23:35Z) https://github.com/owlcs/owlapi
